Move_SEC in Isar style

Move_SEC.thy
@@ -2,16 +2,18 @@ theory Move_SEC
   imports Move CRDT.Network
 begin
 
+section \<open>Strong Eventual Consistency\<close>
+
 definition apply_op' :: \<open>('t::{linorder}, 'n, 'm) operation \<Rightarrow> ('t, 'n, 'm) state \<rightharpoonup> ('t, 'n, 'm) state\<close> where
   \<open>apply_op' x s \<equiv> case s of (log, tree) \<Rightarrow>
     if unique_parent tree \<and> distinct (map log_time log @ [move_time x]) then
       Some (apply_op x s)
     else None\<close>
 
-fun valid_move_opers :: "('t, 'n, 'm) state \<Rightarrow> 't \<times>('t, 'n, 'm) operation \<Rightarrow> bool" where
+fun valid_move_opers :: \<open>('t, 'n, 'm) state \<Rightarrow> 't \<times>('t, 'n, 'm) operation \<Rightarrow> bool\<close> where
   \<open>valid_move_opers _ (i, Move t _ _ _) = (i = t)\<close>
 
-locale move = network_with_constrained_ops _ "apply_op'" "([], {})" valid_move_opers
+locale move = network_with_constrained_ops _ apply_op' \<open>([], {})\<close> valid_move_opers
 begin
 
 lemma kleisli_apply_op' [iff]:
@@ -97,178 +99,189 @@ lemma concurrent_operations_commute:
   using assms by (clarsimp simp add: hb.concurrent_ops_commute_def) (unfold interp_msg_def; simp)
 
 corollary apply_operations_Snoc2:
-  "hb.apply_operations (xs @ [x]) s = (hb.apply_operations xs \<rhd> interp_msg x) s"
+  \<open>hb.apply_operations (xs @ [x]) s = (hb.apply_operations xs \<rhd> interp_msg x) s\<close>
   using hb.apply_operations_Snoc by auto
 
 lemma unique_parent_empty[simp]:
-  shows "unique_parent {}"
+  shows \<open>unique_parent {}\<close>
   by (auto simp: unique_parent_def)
 
 lemma log_tree_invariant:
-  assumes "xs prefix of i"  "apply_operations xs = Some (log, tree)"
-  shows   "distinct (map log_time log) \<and> unique_parent tree"
+  assumes \<open>xs prefix of i\<close>  \<open>apply_operations xs = Some (log, tree)\<close>
+  shows   \<open>distinct (map log_time log) \<and> unique_parent tree\<close>
 using assms proof (induct xs arbitrary: log tree rule: rev_induct, clarsimp)
   case (snoc x xs)
-  hence "apply_operations xs \<noteq> None"
+  hence \<open>apply_operations xs \<noteq> None\<close>
     by (case_tac x; clarsimp simp: apply_operations_def node_deliver_messages_append kleisli_def)
        (metis (no_types, hide_lams) bind_eq_Some_conv surj_pair)
-  then obtain log1 tree1 where *: "apply_operations xs = Some (log1, tree1)"
+  then obtain log1 tree1 where *: \<open>apply_operations xs = Some (log1, tree1)\<close>
     by auto
-  moreover have "xs prefix of i"
+  moreover have \<open>xs prefix of i\<close>
     using snoc.prems(1) by blast
-  ultimately have **: "distinct (map log_time log1)" "unique_parent tree1"
+  ultimately have **: \<open>distinct (map log_time log1)\<close> \<open>unique_parent tree1\<close>
     using snoc.hyps by blast+
   show ?case
   proof (case_tac x)
-    fix m assume "x = Broadcast m"
-    hence "apply_operations (xs @ [x]) = apply_operations xs"
+    fix m assume \<open>x = Broadcast m\<close>
+    hence \<open>apply_operations (xs @ [x]) = apply_operations xs\<close>
       by simp
-    thus "distinct (map log_time log) \<and> unique_parent tree"
+    thus \<open>distinct (map log_time log) \<and> unique_parent tree\<close>
       using \<open>xs prefix of i\<close> snoc.hyps snoc.prems(2) by presburger
   next
-    fix m assume 1: "x = Deliver m"
+    fix m assume 1: \<open>x = Deliver m\<close>
     obtain t oper where 2: "m = (t, oper)"
       by force
-    hence "interp_msg (t, oper) (log1, tree1) = Some (log, tree)"
+    hence \<open>interp_msg (t, oper) (log1, tree1) = Some (log, tree)\<close>
       using \<open>apply_operations xs = Some (log1, tree1)\<close> snoc.prems(2) 1 2 by simp
-    hence 4: "apply_op' oper (log1, tree1) = Some (log, tree)"
+    hence 4: \<open>apply_op' oper (log1, tree1) = Some (log, tree)\<close>
       by (clarsimp simp: interp_msg_def apply_op'_def)
-    hence "distinct ((map log_time log1) @ [move_time oper])"
+    hence \<open>distinct ((map log_time log1) @ [move_time oper])\<close>
       by (clarsimp simp: apply_op'_def) (meson option.distinct(1))
-    moreover hence 5: "apply_op oper (log1, tree1) = (log, tree)"
+    moreover hence 5: \<open>apply_op oper (log1, tree1) = (log, tree)\<close>
       using 4 ** by (clarsimp simp: apply_op'_def)
-    ultimately have "distinct (map log_time log)"
-      apply (case_tac oper, clarsimp)
-      apply (rule apply_op_timestampI1, assumption)
-      by (clarsimp simp add: \<open>distinct (map log_time log1)\<close>)
-    thus "distinct (map log_time log) \<and> unique_parent tree"
+    ultimately have \<open>distinct (map log_time log)\<close>
+      by (case_tac oper, clarsimp) (rule apply_op_timestampI1, assumption, clarsimp)
+    thus \<open>distinct (map log_time log) \<and> unique_parent tree\<close>
       using ** 5 apply_op_unique_parent by blast
   qed
 qed
 
 definition indices :: "('id \<times> ('id, 'v, 'm) operation) event list \<Rightarrow> 'id list" where
-  "indices xs \<equiv> List.map_filter (\<lambda>x. case x of Deliver (i, _) \<Rightarrow> Some i | _ \<Rightarrow> None) xs"
+  \<open>indices xs \<equiv> List.map_filter (\<lambda>x. case x of Deliver (i, _) \<Rightarrow> Some i | _ \<Rightarrow> None) xs\<close>
 
 lemma indices_Nil [simp]:
-  shows "indices [] = []"
+  shows \<open>indices [] = []\<close>
 by(auto simp: indices_def map_filter_def)
 
 lemma indices_append [simp]:
-  shows "indices (xs@ys) = indices xs @ indices ys"
+  shows \<open>indices (xs@ys) = indices xs @ indices ys\<close>
 by(auto simp: indices_def map_filter_def)
 
 lemma indices_Broadcast_singleton [simp]:
-  shows "indices [Broadcast b] = []"
+  shows \<open>indices [Broadcast b] = []\<close>
 by(auto simp: indices_def map_filter_def)
 
 lemma indices_Deliver_Insert [simp]:
-  shows "indices [Deliver (i, x)] = [i]"
+  shows \<open>indices [Deliver (i, x)] = [i]\<close>
   by(auto simp: indices_def map_filter_def)
 
 lemma idx_in_elem[intro]:
-  assumes "Deliver (i, x) \<in> set xs"
-  shows   "i \<in> set (indices xs)"
+  assumes \<open>Deliver (i, x) \<in> set xs\<close>
+  shows   \<open>i \<in> set (indices xs)\<close>
 using assms by(induction xs, auto simp add: indices_def map_filter_def)
 
 lemma valid_move_oper_delivered:
-  assumes "xs@[Deliver (t, oper)] prefix of i"
-  shows "move_time oper = t"
+  assumes \<open>xs@[Deliver (t, oper)] prefix of i\<close>
+  shows   \<open>move_time oper = t\<close>
 by (metis assms deliver_in_prefix_is_valid in_set_conv_decomp operation.set_cases(1) operation.set_sel(1) valid_move_opers.simps)
 
+find_theorems "apply_operations (?xs @ [?x])"
+
 lemma apply_opers_idx_elems:
-  assumes "xs prefix of i" "apply_operations xs = Some (log, tree)"
-  shows "set (map log_time log) = set (indices xs)"
-  using assms apply (induction xs arbitrary: log tree rule: rev_induct)
-   apply force
-  apply (subgoal_tac "xs prefix of i")
-  prefer 2 apply force
-  apply (case_tac x)
-   apply clarsimp
-  apply (case_tac "apply_operations xs")
-  apply force
-  apply (clarsimp simp: interp_msg_def apply_op'_def)
-  apply (subgoal_tac "unique_parent ba \<and> distinct (map log_time aa)")
-   prefer 2
-   apply (simp add: log_tree_invariant)
-  apply (case_tac "move_time b \<notin> set (indices xs)")
-  prefer 2
-   apply force
-  apply clarsimp
-  apply (case_tac b)
-  apply clarsimp
-  apply (subgoal_tac "set (map log_time log) = {x1} \<union> set (map log_time aa)")
-   prefer 2
-   apply (rule apply_op_timestampI2)
-    apply assumption
-   apply force
-  apply (subgoal_tac "a = x1")
-   apply force
-  using valid_move_oper_delivered
-  by (metis operation.sel(1))
+  assumes \<open>xs prefix of i\<close> \<open>apply_operations xs = Some (log, tree)\<close>
+  shows   \<open>set (map log_time log) = set (indices xs)\<close>
+using assms proof (induction xs arbitrary: log tree rule: rev_induct, force)
+  case (snoc x xs)
+  moreover have prefix: \<open>xs prefix of i\<close>
+    using snoc by force
+  ultimately show ?case
+  proof (cases x, force)
+    case (Deliver m)
+    then obtain t oper where m: \<open>m = (t, oper)\<close>
+      by fastforce
+    from Deliver and snoc show ?thesis
+    proof (cases \<open>apply_operations xs\<close>, force)
+      case (Some st)
+      then obtain log' tree' where st: \<open>st = (log', tree')\<close>
+        by (meson surj_pair)
+      have set_indices: \<open>log_time ` set log' = set (indices xs)\<close>
+        using Some prefix snoc.IH st by auto
+      hence *:\<open>unique_parent tree' \<and> distinct (map log_time log')\<close>
+        using st Some prefix by (simp add: log_tree_invariant)
+      hence **: \<open>apply_operations (xs @ [x]) =
+             (if move_time oper \<notin> set (indices xs) then Some (apply_op (snd (t, oper)) (log', tree'))
+             else None)\<close>
+        using Deliver Some st m set_indices by (auto simp: interp_msg_def apply_op'_def)
+      hence ***: \<open>move_time oper \<notin> set (indices xs)\<close>
+        using snoc.prems(2) by auto
+      obtain t' p m c where oper: \<open>oper = Move t' p m c\<close>
+        using operation.exhaust by blast
+      hence \<open>t = t'\<close>
+        using valid_move_oper_delivered Deliver m snoc.prems(1) by fastforce
+      hence \<open>apply_op (Move t p m c) (log', tree') = (log, tree)\<close>
+        by (metis ** oper option.discI option.simps(1) prod.sel(2) snoc.prems(2))
+      hence \<open>set (map log_time log) = {t} \<union> set (map log_time log')\<close>
+        apply (rule apply_op_timestampI2)
+        using Deliver * *** m set_indices snoc.prems(1) valid_move_oper_delivered by auto
+      thus ?thesis
+        using Deliver m set_indices by (clarsimp simp: interp_msg_def apply_op'_def)
+    qed
+  qed                                
+qed
 
 lemma indices_distinct_aux:
-  assumes "xs @ [Deliver (a, b)] prefix of i"
-    shows "a \<notin> set (indices xs)"
+  assumes \<open>xs @ [Deliver (a, b)] prefix of i\<close>
+    shows \<open>a \<notin> set (indices xs)\<close>
 proof 
-  have 1: "xs prefix of i"
+  have 1: \<open>xs prefix of i\<close>
     using assms by force
-  assume "a \<in> set (indices xs)"
-  hence "\<exists>x. Deliver (a, x) \<in> set xs"
+  assume \<open>a \<in> set (indices xs)\<close>
+  hence \<open>\<exists>x. Deliver (a, x) \<in> set xs\<close>
     by (clarsimp simp: indices_def map_filter_def, case_tac x; force)
-  then obtain c where 2: "Deliver (a, c) \<in> set xs"
+  then obtain c where 2: \<open>Deliver (a, c) \<in> set xs\<close>
     by auto
-  moreover then obtain j where "Broadcast (a, c) \<in> set (history j)"
+  moreover then obtain j where \<open>Broadcast (a, c) \<in> set (history j)\<close>
     using 1 delivery_has_a_cause prefix_elem_to_carriers by blast
-  moreover obtain k where "Broadcast (a, b) \<in> set (history k)"
+  moreover obtain k where \<open>Broadcast (a, b) \<in> set (history k)\<close>
     by (meson assms delivery_has_a_cause in_set_conv_decomp prefix_elem_to_carriers)
-  ultimately have "b = c"
+  ultimately have \<open>b = c\<close>
     by (metis fst_conv network.msg_id_unique network_axioms old.prod.inject)
-  hence "\<not> distinct (xs @ [Deliver (a, b)])"
+  hence \<open>\<not> distinct (xs @ [Deliver (a, b)])\<close>
     by (simp add: 2)
-  thus "False"
+  thus \<open>False\<close>
     using assms prefix_distinct by blast
 qed
 
 
 lemma indices_distinct:
-  assumes "xs prefix of i"
-  shows   "distinct (indices xs)"
+  assumes \<open>xs prefix of i\<close>
+  shows   \<open>distinct (indices xs)\<close>
 using assms proof (induct xs rule: rev_induct, clarsimp)
   case (snoc x xs)
-  hence "xs prefix of i"
+  hence \<open>xs prefix of i\<close>
     by force
-  moreover hence "distinct (indices xs)"
+  moreover hence \<open>distinct (indices xs)\<close>
     by (simp add: snoc.hyps)
   ultimately show ?case
     using indices_distinct_aux snoc.prems by (case_tac x; force)
 qed
 
 lemma log_time_invariant:
-  assumes "xs@[Deliver (t, oper)] prefix of i"  "apply_operations xs = Some (log, tree)"
-  shows   "move_time oper \<notin> set (map log_time log)"
+  assumes \<open>xs@[Deliver (t, oper)] prefix of i\<close>  \<open>apply_operations xs = Some (log, tree)\<close>
+  shows   \<open>move_time oper \<notin> set (map log_time log)\<close>
 proof -
-  have "xs prefix of i"
+  have \<open>xs prefix of i\<close>
     using assms by force
-  have "move_time oper = t"
+  have \<open>move_time oper = t\<close>
     using assms valid_move_oper_delivered by auto
-  moreover have "indices (xs @ [Deliver (t, oper)]) = indices xs @ [t]"
+  moreover have \<open>indices (xs @ [Deliver (t, oper)]) = indices xs @ [t]\<close>
     by simp
-  moreover have "distinct (indices (xs @ [Deliver (t, oper)]))"
+  moreover have \<open>distinct (indices (xs @ [Deliver (t, oper)]))\<close>
     using assms indices_distinct by blast
   ultimately show ?thesis
     using apply_opers_idx_elems assms indices_distinct_aux by blast
 qed    
 
 lemma apply_operations_never_fails:
-  assumes "xs prefix of i"
-  shows "apply_operations xs \<noteq> None"
+  assumes \<open>xs prefix of i\<close>
+  shows   \<open>apply_operations xs \<noteq> None\<close>
 using assms proof(induct xs rule: rev_induct, clarsimp)
   case (snoc x xs)
-  hence "apply_operations xs \<noteq> None"
+  hence \<open>apply_operations xs \<noteq> None\<close>
     by blast
-  then obtain log1 tree1 where *: "apply_operations xs = Some (log1, tree1)"
+  then obtain log1 tree1 where *: \<open>apply_operations xs = Some (log1, tree1)\<close>
     by auto
-  moreover hence "distinct (map log_time log1) \<and> unique_parent tree1"
+  moreover hence \<open>distinct (map log_time log1) \<and> unique_parent tree1\<close>
     using log_tree_invariant snoc.prems by blast
   ultimately show ?case
     using log_time_invariant snoc.prems
@@ -276,36 +289,36 @@ using assms proof(induct xs rule: rev_induct, clarsimp)
 qed
 
 sublocale sec: strong_eventual_consistency weak_hb hb interp_msg
-  "\<lambda>os. \<exists>xs i. xs prefix of i \<and> node_deliver_messages xs = os" "([], {})"
+  \<open>\<lambda>os. \<exists>xs i. xs prefix of i \<and> node_deliver_messages xs = os\<close> \<open>([], {})\<close>
 proof (standard; clarsimp)
   fix xsa i
-  assume "xsa prefix of i"
-  thus "hb.hb_consistent (node_deliver_messages xsa)"
+  assume \<open>xsa prefix of i\<close>
+  thus \<open>hb.hb_consistent (node_deliver_messages xsa)\<close>
     by(auto simp add: hb_consistent_prefix)
 next
   fix xsa i
-  assume "xsa prefix of i"
-  thus "distinct (node_deliver_messages xsa)"
+  assume \<open>xsa prefix of i\<close>
+  thus \<open>distinct (node_deliver_messages xsa)\<close>
     by(auto simp add: node_deliver_messages_distinct)
 next
   fix xsa i
-  assume "xsa prefix of i"
-  thus "hb.concurrent_ops_commute (node_deliver_messages xsa)"
+  assume \<open>xsa prefix of i\<close>
+  thus \<open>hb.concurrent_ops_commute (node_deliver_messages xsa)\<close>
     by(auto simp add: concurrent_operations_commute)
 next
   fix xs a b state xsa x
-  assume "hb.apply_operations xs ([], {}) = Some state"
-         "node_deliver_messages xsa = xs @ [(a, b)]"
-         "xsa prefix of x"
-  moreover hence "apply_operations xsa \<noteq> None"
+  assume \<open>hb.apply_operations xs ([], {}) = Some state\<close>
+         \<open>node_deliver_messages xsa = xs @ [(a, b)]\<close>
+         \<open>xsa prefix of x\<close>
+  moreover hence \<open>apply_operations xsa \<noteq> None\<close>
     using apply_operations_never_fails by blast
-  ultimately show "\<exists>ab bb. interp_msg (a, b) state = Some (ab, bb)"
+  ultimately show \<open>\<exists>ab bb. interp_msg (a, b) state = Some (ab, bb)\<close>
     by (clarsimp simp: apply_operations_def kleisli_def)
 next
   fix xs a b xsa x
-  assume "node_deliver_messages xsa = xs @ [(a, b)]"
-    and "xsa prefix of x"
-  thus "\<exists>xsa. (\<exists>x. xsa prefix of x) \<and> node_deliver_messages xsa = xs"
+  assume \<open>node_deliver_messages xsa = xs @ [(a, b)]\<close>
+    and  \<open>xsa prefix of x\<close>
+  thus \<open>\<exists>xsa. (\<exists>x. xsa prefix of x) \<and> node_deliver_messages xsa = xs\<close>
     using drop_last_message by blast
 qed
 
