ROOT
@@ -1,7 +1,9 @@
-session "CRDT-Tree" = "HOL" +
-  options [document = pdf, document_output = "output"]
+chapter AFP
+session "CRDT-Tree" (AFP) = "HOL" +
+  options [timeout = 600, document = pdf, document_output = "output"]
   theories
     Move
+    Move_SEC
   document_files
     "root.tex"
     "root.bib"
